Prefix(:=<http://www.semanticweb.org/dani2/ontologies/2024/3/PAC2_2/>)
Prefix(owl:=<http://www.w3.org/2002/07/owl#>)
Prefix(rdf:=<http://www.w3.org/1999/02/22-rdf-syntax-ns#>)
Prefix(xml:=<http://www.w3.org/XML/1998/namespace>)
Prefix(xsd:=<http://www.w3.org/2001/XMLSchema#>)
Prefix(rdfs:=<http://www.w3.org/2000/01/rdf-schema#>)


Ontology(<http://www.semanticweb.org/dani2/ontologies/2024/3/PAC2_2>
Annotation(rdfs:comment "Author: Daniel Soriano Pons
University: Universitat Oberta de Catalunya")

Declaration(Class(<http://www.semanticweb.org/dani2/ontologies/2024/3/PAC2_2#Address>))
Declaration(Class(<http://www.semanticweb.org/dani2/ontologies/2024/3/PAC2_2#Age>))
Declaration(Class(<http://www.semanticweb.org/dani2/ontologies/2024/3/PAC2_2#Airline_Company>))
Declaration(Class(<http://www.semanticweb.org/dani2/ontologies/2024/3/PAC2_2#Airplane>))
Declaration(Class(<http://www.semanticweb.org/dani2/ontologies/2024/3/PAC2_2#Ariplane_Fleet>))
Declaration(Class(<http://www.semanticweb.org/dani2/ontologies/2024/3/PAC2_2#BusinessClass>))
Declaration(Class(<http://www.semanticweb.org/dani2/ontologies/2024/3/PAC2_2#Business_Traveller>))
Declaration(Class(<http://www.semanticweb.org/dani2/ontologies/2024/3/PAC2_2#City>))
Declaration(Class(<http://www.semanticweb.org/dani2/ontologies/2024/3/PAC2_2#Company>))
Declaration(Class(<http://www.semanticweb.org/dani2/ontologies/2024/3/PAC2_2#Continent>))
Declaration(Class(<http://www.semanticweb.org/dani2/ontologies/2024/3/PAC2_2#Country>))
Declaration(Class(<http://www.semanticweb.org/dani2/ontologies/2024/3/PAC2_2#Couple_Leisure>))
Declaration(Class(<http://www.semanticweb.org/dani2/ontologies/2024/3/PAC2_2#Customer>))
Declaration(Class(<http://www.semanticweb.org/dani2/ontologies/2024/3/PAC2_2#Customer_Flight_Review>))
Declaration(Class(<http://www.semanticweb.org/dani2/ontologies/2024/3/PAC2_2#Customer_Review>))
Declaration(Class(<http://www.semanticweb.org/dani2/ontologies/2024/3/PAC2_2#Date>))
Declaration(Class(<http://www.semanticweb.org/dani2/ontologies/2024/3/PAC2_2#Day>))
Declaration(Class(<http://www.semanticweb.org/dani2/ontologies/2024/3/PAC2_2#Description>))
Declaration(Class(<http://www.semanticweb.org/dani2/ontologies/2024/3/PAC2_2#Destination>))
Declaration(Class(<http://www.semanticweb.org/dani2/ontologies/2024/3/PAC2_2#EconomyClass>))
Declaration(Class(<http://www.semanticweb.org/dani2/ontologies/2024/3/PAC2_2#Family_Leisure>))
Declaration(Class(<http://www.semanticweb.org/dani2/ontologies/2024/3/PAC2_2#FirstClass>))
Declaration(Class(<http://www.semanticweb.org/dani2/ontologies/2024/3/PAC2_2#Flight>))
Declaration(Class(<http://www.semanticweb.org/dani2/ontologies/2024/3/PAC2_2#Flight_Date>))
Declaration(Class(<http://www.semanticweb.org/dani2/ontologies/2024/3/PAC2_2#Flight_Rate>))
Declaration(Class(<http://www.semanticweb.org/dani2/ontologies/2024/3/PAC2_2#Flight_Service>))
Declaration(Class(<http://www.semanticweb.org/dani2/ontologies/2024/3/PAC2_2#Leisure_Traveller>))
Declaration(Class(<http://www.semanticweb.org/dani2/ontologies/2024/3/PAC2_2#Month>))
Declaration(Class(<http://www.semanticweb.org/dani2/ontologies/2024/3/PAC2_2#Nationality>))
Declaration(Class(<http://www.semanticweb.org/dani2/ontologies/2024/3/PAC2_2#No>))
Declaration(Class(<http://www.semanticweb.org/dani2/ontologies/2024/3/PAC2_2#Origin>))
Declaration(Class(<http://www.semanticweb.org/dani2/ontologies/2024/3/PAC2_2#Owner>))
Declaration(Class(<http://www.semanticweb.org/dani2/ontologies/2024/3/PAC2_2#Person>))
Declaration(Class(<http://www.semanticweb.org/dani2/ontologies/2024/3/PAC2_2#PremiunEconomyClass>))
Declaration(Class(<http://www.semanticweb.org/dani2/ontologies/2024/3/PAC2_2#Professional_Review>))
Declaration(Class(<http://www.semanticweb.org/dani2/ontologies/2024/3/PAC2_2#Recommend>))
Declaration(Class(<http://www.semanticweb.org/dani2/ontologies/2024/3/PAC2_2#Review>))
Declaration(Class(<http://www.semanticweb.org/dani2/ontologies/2024/3/PAC2_2#Review_Owner>))
Declaration(Class(<http://www.semanticweb.org/dani2/ontologies/2024/3/PAC2_2#SeatClass>))
Declaration(Class(<http://www.semanticweb.org/dani2/ontologies/2024/3/PAC2_2#Services>))
Declaration(Class(<http://www.semanticweb.org/dani2/ontologies/2024/3/PAC2_2#Solo_Leisure>))
Declaration(Class(<http://www.semanticweb.org/dani2/ontologies/2024/3/PAC2_2#Ticket>))
Declaration(Class(<http://www.semanticweb.org/dani2/ontologies/2024/3/PAC2_2#Title>))
Declaration(Class(<http://www.semanticweb.org/dani2/ontologies/2024/3/PAC2_2#Traveller>))
Declaration(Class(<http://www.semanticweb.org/dani2/ontologies/2024/3/PAC2_2#Vehicle>))
Declaration(Class(<http://www.semanticweb.org/dani2/ontologies/2024/3/PAC2_2#Year>))
Declaration(Class(<http://www.semanticweb.org/dani2/ontologies/2024/3/PAC2_2#Yes>))
Declaration(Class(<http://www.semanticweb.org/dani2/ontologies/2024/3/PAC2_2#N/A>))
Declaration(ObjectProperty(<http://www.semanticweb.org/dani2/ontologies/2024/3/PAC2_2#hasAirplane>))
Declaration(ObjectProperty(<http://www.semanticweb.org/dani2/ontologies/2024/3/PAC2_2#hasCustomer>))
Declaration(ObjectProperty(<http://www.semanticweb.org/dani2/ontologies/2024/3/PAC2_2#hasDestination>))
Declaration(ObjectProperty(<http://www.semanticweb.org/dani2/ontologies/2024/3/PAC2_2#hasFlight>))
Declaration(ObjectProperty(<http://www.semanticweb.org/dani2/ontologies/2024/3/PAC2_2#hasFlightDate>))
Declaration(ObjectProperty(<http://www.semanticweb.org/dani2/ontologies/2024/3/PAC2_2#hasNationality>))
Declaration(ObjectProperty(<http://www.semanticweb.org/dani2/ontologies/2024/3/PAC2_2#hasOrigin>))
Declaration(ObjectProperty(<http://www.semanticweb.org/dani2/ontologies/2024/3/PAC2_2#hasOwner>))
Declaration(ObjectProperty(<http://www.semanticweb.org/dani2/ontologies/2024/3/PAC2_2#hasSeatClass>))
Declaration(DataProperty(<http://www.semanticweb.org/dani2/ontologies/2024/3/PAC2_2#hasAge>))
Declaration(DataProperty(<http://www.semanticweb.org/dani2/ontologies/2024/3/PAC2_2#hasRating>))
Declaration(NamedIndividual(<http://www.semanticweb.org/dani2/ontologies/2024/3/PAC2_2#Albert>))
Declaration(NamedIndividual(<http://www.semanticweb.org/dani2/ontologies/2024/3/PAC2_2#Alicante>))
Declaration(NamedIndividual(<http://www.semanticweb.org/dani2/ontologies/2024/3/PAC2_2#Boeing_737>))
Declaration(NamedIndividual(<http://www.semanticweb.org/dani2/ontologies/2024/3/PAC2_2#David>))
Declaration(NamedIndividual(<http://www.semanticweb.org/dani2/ontologies/2024/3/PAC2_2#Marta>))
Declaration(NamedIndividual(<http://www.semanticweb.org/dani2/ontologies/2024/3/PAC2_2#Ryanair>))
Declaration(NamedIndividual(<http://www.semanticweb.org/dani2/ontologies/2024/3/PAC2_2#Seat13B>))
Declaration(NamedIndividual(<http://www.semanticweb.org/dani2/ontologies/2024/3/PAC2_2#Seat2A>))
Declaration(NamedIndividual(<http://www.semanticweb.org/dani2/ontologies/2024/3/PAC2_2#Standsted>))
Declaration(NamedIndividual(<http://www.semanticweb.org/dani2/ontologies/2024/3/PAC2_2#13/12/2022>))
Declaration(NamedIndividual(<http://www.semanticweb.org/dani2/ontologies/2024/3/PAC2_2#Boeing737_Albacete_Standsted_13/12/22>))
Declaration(AnnotationProperty(rdfs:sameAs))

############################
#   Object Properties
############################

# Object Property: <http://www.semanticweb.org/dani2/ontologies/2024/3/PAC2_2#hasAirplane> (<http://www.semanticweb.org/dani2/ontologies/2024/3/PAC2_2#hasAirplane>)

ObjectPropertyDomain(<http://www.semanticweb.org/dani2/ontologies/2024/3/PAC2_2#hasAirplane> <http://www.semanticweb.org/dani2/ontologies/2024/3/PAC2_2#Flight>)
ObjectPropertyRange(<http://www.semanticweb.org/dani2/ontologies/2024/3/PAC2_2#hasAirplane> <http://www.semanticweb.org/dani2/ontologies/2024/3/PAC2_2#Airplane>)

# Object Property: <http://www.semanticweb.org/dani2/ontologies/2024/3/PAC2_2#hasCustomer> (hasCustomer)

AnnotationAssertion(rdfs:comment <http://www.semanticweb.org/dani2/ontologies/2024/3/PAC2_2#hasCustomer> "Indicates the customers in the flight")
AnnotationAssertion(rdfs:label <http://www.semanticweb.org/dani2/ontologies/2024/3/PAC2_2#hasCustomer> "hasCustomer")
InverseObjectProperties(<http://www.semanticweb.org/dani2/ontologies/2024/3/PAC2_2#hasCustomer> <http://www.semanticweb.org/dani2/ontologies/2024/3/PAC2_2#hasFlight>)
ObjectPropertyDomain(<http://www.semanticweb.org/dani2/ontologies/2024/3/PAC2_2#hasCustomer> <http://www.semanticweb.org/dani2/ontologies/2024/3/PAC2_2#Flight>)
ObjectPropertyRange(<http://www.semanticweb.org/dani2/ontologies/2024/3/PAC2_2#hasCustomer> <http://www.semanticweb.org/dani2/ontologies/2024/3/PAC2_2#Traveller>)

# Object Property: <http://www.semanticweb.org/dani2/ontologies/2024/3/PAC2_2#hasDestination> (hasDestination)

AnnotationAssertion(rdfs:comment <http://www.semanticweb.org/dani2/ontologies/2024/3/PAC2_2#hasDestination> "The city of destination of the flight")
AnnotationAssertion(rdfs:label <http://www.semanticweb.org/dani2/ontologies/2024/3/PAC2_2#hasDestination> "hasDestination")
FunctionalObjectProperty(<http://www.semanticweb.org/dani2/ontologies/2024/3/PAC2_2#hasDestination>)
ObjectPropertyDomain(<http://www.semanticweb.org/dani2/ontologies/2024/3/PAC2_2#hasDestination> <http://www.semanticweb.org/dani2/ontologies/2024/3/PAC2_2#Flight>)
ObjectPropertyRange(<http://www.semanticweb.org/dani2/ontologies/2024/3/PAC2_2#hasDestination> <http://www.semanticweb.org/dani2/ontologies/2024/3/PAC2_2#City>)

# Object Property: <http://www.semanticweb.org/dani2/ontologies/2024/3/PAC2_2#hasFlight> (hasFlight)

AnnotationAssertion(rdfs:comment <http://www.semanticweb.org/dani2/ontologies/2024/3/PAC2_2#hasFlight> "Indicates the flight of the passenger.")
AnnotationAssertion(rdfs:label <http://www.semanticweb.org/dani2/ontologies/2024/3/PAC2_2#hasFlight> "hasFlight")
ObjectPropertyDomain(<http://www.semanticweb.org/dani2/ontologies/2024/3/PAC2_2#hasFlight> <http://www.semanticweb.org/dani2/ontologies/2024/3/PAC2_2#Customer>)
ObjectPropertyRange(<http://www.semanticweb.org/dani2/ontologies/2024/3/PAC2_2#hasFlight> <http://www.semanticweb.org/dani2/ontologies/2024/3/PAC2_2#Flight>)

# Object Property: <http://www.semanticweb.org/dani2/ontologies/2024/3/PAC2_2#hasFlightDate> (hasFlightDate)

AnnotationAssertion(rdfs:comment <http://www.semanticweb.org/dani2/ontologies/2024/3/PAC2_2#hasFlightDate> "Date of flight")
AnnotationAssertion(rdfs:label <http://www.semanticweb.org/dani2/ontologies/2024/3/PAC2_2#hasFlightDate> "hasFlightDate")
ObjectPropertyDomain(<http://www.semanticweb.org/dani2/ontologies/2024/3/PAC2_2#hasFlightDate> <http://www.semanticweb.org/dani2/ontologies/2024/3/PAC2_2#Flight>)
ObjectPropertyRange(<http://www.semanticweb.org/dani2/ontologies/2024/3/PAC2_2#hasFlightDate> <http://www.semanticweb.org/dani2/ontologies/2024/3/PAC2_2#Date>)

# Object Property: <http://www.semanticweb.org/dani2/ontologies/2024/3/PAC2_2#hasNationality> (hasNationality)

AnnotationAssertion(rdfs:comment <http://www.semanticweb.org/dani2/ontologies/2024/3/PAC2_2#hasNationality> "Country of birth of the person")
AnnotationAssertion(rdfs:label <http://www.semanticweb.org/dani2/ontologies/2024/3/PAC2_2#hasNationality> "hasNationality")
ObjectPropertyDomain(<http://www.semanticweb.org/dani2/ontologies/2024/3/PAC2_2#hasNationality> <http://www.semanticweb.org/dani2/ontologies/2024/3/PAC2_2#Person>)
ObjectPropertyRange(<http://www.semanticweb.org/dani2/ontologies/2024/3/PAC2_2#hasNationality> <http://www.semanticweb.org/dani2/ontologies/2024/3/PAC2_2#Country>)

# Object Property: <http://www.semanticweb.org/dani2/ontologies/2024/3/PAC2_2#hasOrigin> (hasOrigin)

AnnotationAssertion(rdfs:comment <http://www.semanticweb.org/dani2/ontologies/2024/3/PAC2_2#hasOrigin> "City of origin of the flight")
AnnotationAssertion(rdfs:label <http://www.semanticweb.org/dani2/ontologies/2024/3/PAC2_2#hasOrigin> "hasOrigin")
FunctionalObjectProperty(<http://www.semanticweb.org/dani2/ontologies/2024/3/PAC2_2#hasOrigin>)
ObjectPropertyDomain(<http://www.semanticweb.org/dani2/ontologies/2024/3/PAC2_2#hasOrigin> <http://www.semanticweb.org/dani2/ontologies/2024/3/PAC2_2#Flight>)
ObjectPropertyRange(<http://www.semanticweb.org/dani2/ontologies/2024/3/PAC2_2#hasOrigin> <http://www.semanticweb.org/dani2/ontologies/2024/3/PAC2_2#City>)

# Object Property: <http://www.semanticweb.org/dani2/ontologies/2024/3/PAC2_2#hasOwner> (hasOwner)

AnnotationAssertion(rdfs:comment <http://www.semanticweb.org/dani2/ontologies/2024/3/PAC2_2#hasOwner> "The owner of the airline in charge of the flight")
AnnotationAssertion(rdfs:label <http://www.semanticweb.org/dani2/ontologies/2024/3/PAC2_2#hasOwner> "hasOwner")
FunctionalObjectProperty(<http://www.semanticweb.org/dani2/ontologies/2024/3/PAC2_2#hasOwner>)
ObjectPropertyDomain(<http://www.semanticweb.org/dani2/ontologies/2024/3/PAC2_2#hasOwner> <http://www.semanticweb.org/dani2/ontologies/2024/3/PAC2_2#Flight>)
ObjectPropertyRange(<http://www.semanticweb.org/dani2/ontologies/2024/3/PAC2_2#hasOwner> <http://www.semanticweb.org/dani2/ontologies/2024/3/PAC2_2#Airline_Company>)

# Object Property: <http://www.semanticweb.org/dani2/ontologies/2024/3/PAC2_2#hasSeatClass> (hasSeatClass)

AnnotationAssertion(rdfs:comment <http://www.semanticweb.org/dani2/ontologies/2024/3/PAC2_2#hasSeatClass> "Indicates the class seat of the passenger")
AnnotationAssertion(rdfs:label <http://www.semanticweb.org/dani2/ontologies/2024/3/PAC2_2#hasSeatClass> "hasSeatClass")
ObjectPropertyDomain(<http://www.semanticweb.org/dani2/ontologies/2024/3/PAC2_2#hasSeatClass> <http://www.semanticweb.org/dani2/ontologies/2024/3/PAC2_2#Customer_Flight_Review>)
ObjectPropertyRange(<http://www.semanticweb.org/dani2/ontologies/2024/3/PAC2_2#hasSeatClass> <http://www.semanticweb.org/dani2/ontologies/2024/3/PAC2_2#SeatClass>)


############################
#   Data Properties
############################

# Data Property: <http://www.semanticweb.org/dani2/ontologies/2024/3/PAC2_2#hasAge> (hasAge)

AnnotationAssertion(rdfs:comment <http://www.semanticweb.org/dani2/ontologies/2024/3/PAC2_2#hasAge> "Indicates the age of the person")
AnnotationAssertion(rdfs:label <http://www.semanticweb.org/dani2/ontologies/2024/3/PAC2_2#hasAge> "hasAge")
SubDataPropertyOf(<http://www.semanticweb.org/dani2/ontologies/2024/3/PAC2_2#hasAge> owl:topDataProperty)
FunctionalDataProperty(<http://www.semanticweb.org/dani2/ontologies/2024/3/PAC2_2#hasAge>)
DataPropertyDomain(<http://www.semanticweb.org/dani2/ontologies/2024/3/PAC2_2#hasAge> <http://www.semanticweb.org/dani2/ontologies/2024/3/PAC2_2#Person>)
DataPropertyRange(<http://www.semanticweb.org/dani2/ontologies/2024/3/PAC2_2#hasAge> xsd:integer)

# Data Property: <http://www.semanticweb.org/dani2/ontologies/2024/3/PAC2_2#hasRating> (hasRating)

AnnotationAssertion(rdfs:comment <http://www.semanticweb.org/dani2/ontologies/2024/3/PAC2_2#hasRating> "Rating of the flight for that customer review")
AnnotationAssertion(rdfs:label <http://www.semanticweb.org/dani2/ontologies/2024/3/PAC2_2#hasRating> "hasRating")
FunctionalDataProperty(<http://www.semanticweb.org/dani2/ontologies/2024/3/PAC2_2#hasRating>)
DataPropertyDomain(<http://www.semanticweb.org/dani2/ontologies/2024/3/PAC2_2#hasRating> <http://www.semanticweb.org/dani2/ontologies/2024/3/PAC2_2#Customer_Flight_Review>)
DataPropertyRange(<http://www.semanticweb.org/dani2/ontologies/2024/3/PAC2_2#hasRating> xsd:integer)



############################
#   Classes
############################

# Class: <http://www.semanticweb.org/dani2/ontologies/2024/3/PAC2_2#Address> (Address)

AnnotationAssertion(rdfs:comment <http://www.semanticweb.org/dani2/ontologies/2024/3/PAC2_2#Address> "Address where the person lives")
AnnotationAssertion(rdfs:label <http://www.semanticweb.org/dani2/ontologies/2024/3/PAC2_2#Address> "Address")
SubClassOf(<http://www.semanticweb.org/dani2/ontologies/2024/3/PAC2_2#Address> <http://www.semanticweb.org/dani2/ontologies/2024/3/PAC2_2#Person>)

# Class: <http://www.semanticweb.org/dani2/ontologies/2024/3/PAC2_2#Age> (<http://www.semanticweb.org/dani2/ontologies/2024/3/PAC2_2#Age>)

SubClassOf(<http://www.semanticweb.org/dani2/ontologies/2024/3/PAC2_2#Age> <http://www.semanticweb.org/dani2/ontologies/2024/3/PAC2_2#Person>)

# Class: <http://www.semanticweb.org/dani2/ontologies/2024/3/PAC2_2#Airline_Company> (Airplane Company)

AnnotationAssertion(rdfs:comment <http://www.semanticweb.org/dani2/ontologies/2024/3/PAC2_2#Airline_Company> "A company or organisation that his main activity is to provide flights using ariplanes")
AnnotationAssertion(rdfs:label <http://www.semanticweb.org/dani2/ontologies/2024/3/PAC2_2#Airline_Company> "Airplane Company")
SubClassOf(<http://www.semanticweb.org/dani2/ontologies/2024/3/PAC2_2#Airline_Company> <http://www.semanticweb.org/dani2/ontologies/2024/3/PAC2_2#Company>)

# Class: <http://www.semanticweb.org/dani2/ontologies/2024/3/PAC2_2#Airplane> (Airplane)

AnnotationAssertion(rdfs:comment <http://www.semanticweb.org/dani2/ontologies/2024/3/PAC2_2#Airplane> "A airplane.")
AnnotationAssertion(rdfs:label <http://www.semanticweb.org/dani2/ontologies/2024/3/PAC2_2#Airplane> "Airplane")
AnnotationAssertion(rdfs:sameAs <http://www.semanticweb.org/dani2/ontologies/2024/3/PAC2_2#Airplane> "https://dbpedia.org/page/Airplane")
SubClassOf(<http://www.semanticweb.org/dani2/ontologies/2024/3/PAC2_2#Airplane> <http://www.semanticweb.org/dani2/ontologies/2024/3/PAC2_2#Vehicle>)

# Class: <http://www.semanticweb.org/dani2/ontologies/2024/3/PAC2_2#Ariplane_Fleet> (Airplane Fleet)

AnnotationAssertion(rdfs:comment <http://www.semanticweb.org/dani2/ontologies/2024/3/PAC2_2#Ariplane_Fleet> "All the airplanes that are owned by the airplane company")
AnnotationAssertion(rdfs:label <http://www.semanticweb.org/dani2/ontologies/2024/3/PAC2_2#Ariplane_Fleet> "Airplane Fleet")
SubClassOf(<http://www.semanticweb.org/dani2/ontologies/2024/3/PAC2_2#Ariplane_Fleet> <http://www.semanticweb.org/dani2/ontologies/2024/3/PAC2_2#Airline_Company>)

# Class: <http://www.semanticweb.org/dani2/ontologies/2024/3/PAC2_2#BusinessClass> (Business Class)

AnnotationAssertion(rdfs:comment <http://www.semanticweb.org/dani2/ontologies/2024/3/PAC2_2#BusinessClass> "Class designed for Business Travelers")
AnnotationAssertion(rdfs:label <http://www.semanticweb.org/dani2/ontologies/2024/3/PAC2_2#BusinessClass> "Business Class")
SubClassOf(<http://www.semanticweb.org/dani2/ontologies/2024/3/PAC2_2#BusinessClass> <http://www.semanticweb.org/dani2/ontologies/2024/3/PAC2_2#SeatClass>)

# Class: <http://www.semanticweb.org/dani2/ontologies/2024/3/PAC2_2#Business_Traveller> (Business Traveller)

AnnotationAssertion(rdfs:comment <http://www.semanticweb.org/dani2/ontologies/2024/3/PAC2_2#Business_Traveller> "Traveller that has business as their purpouse.")
AnnotationAssertion(rdfs:label <http://www.semanticweb.org/dani2/ontologies/2024/3/PAC2_2#Business_Traveller> "Business Traveller")
SubClassOf(<http://www.semanticweb.org/dani2/ontologies/2024/3/PAC2_2#Business_Traveller> <http://www.semanticweb.org/dani2/ontologies/2024/3/PAC2_2#Traveller>)
DisjointClasses(<http://www.semanticweb.org/dani2/ontologies/2024/3/PAC2_2#Business_Traveller> <http://www.semanticweb.org/dani2/ontologies/2024/3/PAC2_2#Leisure_Traveller>)

# Class: <http://www.semanticweb.org/dani2/ontologies/2024/3/PAC2_2#City> (City)

AnnotationAssertion(rdfs:comment <http://www.semanticweb.org/dani2/ontologies/2024/3/PAC2_2#City> "A city")
AnnotationAssertion(rdfs:label <http://www.semanticweb.org/dani2/ontologies/2024/3/PAC2_2#City> "City")
AnnotationAssertion(rdfs:sameAs <http://www.semanticweb.org/dani2/ontologies/2024/3/PAC2_2#City> "https://dbpedia.org/page/City")
SubClassOf(<http://www.semanticweb.org/dani2/ontologies/2024/3/PAC2_2#City> <http://www.semanticweb.org/dani2/ontologies/2024/3/PAC2_2#Country>)

# Class: <http://www.semanticweb.org/dani2/ontologies/2024/3/PAC2_2#Company> (Company)

AnnotationAssertion(rdfs:comment <http://www.semanticweb.org/dani2/ontologies/2024/3/PAC2_2#Company> "A company or organisation")
AnnotationAssertion(rdfs:label <http://www.semanticweb.org/dani2/ontologies/2024/3/PAC2_2#Company> "Company")

# Class: <http://www.semanticweb.org/dani2/ontologies/2024/3/PAC2_2#Continent> (Continent)

AnnotationAssertion(rdfs:comment <http://www.semanticweb.org/dani2/ontologies/2024/3/PAC2_2#Continent> "A continent")
AnnotationAssertion(rdfs:label <http://www.semanticweb.org/dani2/ontologies/2024/3/PAC2_2#Continent> "Continent")

# Class: <http://www.semanticweb.org/dani2/ontologies/2024/3/PAC2_2#Country> (Country)

AnnotationAssertion(rdfs:comment <http://www.semanticweb.org/dani2/ontologies/2024/3/PAC2_2#Country> "A country")
AnnotationAssertion(rdfs:label <http://www.semanticweb.org/dani2/ontologies/2024/3/PAC2_2#Country> "Country")
SubClassOf(<http://www.semanticweb.org/dani2/ontologies/2024/3/PAC2_2#Country> <http://www.semanticweb.org/dani2/ontologies/2024/3/PAC2_2#Continent>)

# Class: <http://www.semanticweb.org/dani2/ontologies/2024/3/PAC2_2#Couple_Leisure> (Couple Leisure)

AnnotationAssertion(rdfs:comment <http://www.semanticweb.org/dani2/ontologies/2024/3/PAC2_2#Couple_Leisure> "Travellers that are travelling as a couple.")
AnnotationAssertion(rdfs:label <http://www.semanticweb.org/dani2/ontologies/2024/3/PAC2_2#Couple_Leisure> "Couple Leisure")
SubClassOf(<http://www.semanticweb.org/dani2/ontologies/2024/3/PAC2_2#Couple_Leisure> <http://www.semanticweb.org/dani2/ontologies/2024/3/PAC2_2#Leisure_Traveller>)
DisjointClasses(<http://www.semanticweb.org/dani2/ontologies/2024/3/PAC2_2#Couple_Leisure> <http://www.semanticweb.org/dani2/ontologies/2024/3/PAC2_2#Family_Leisure>)
DisjointClasses(<http://www.semanticweb.org/dani2/ontologies/2024/3/PAC2_2#Couple_Leisure> <http://www.semanticweb.org/dani2/ontologies/2024/3/PAC2_2#Solo_Leisure>)

# Class: <http://www.semanticweb.org/dani2/ontologies/2024/3/PAC2_2#Customer> (Customer)

AnnotationAssertion(rdfs:comment <http://www.semanticweb.org/dani2/ontologies/2024/3/PAC2_2#Customer> "Person that is taking  the flight.")
AnnotationAssertion(rdfs:label <http://www.semanticweb.org/dani2/ontologies/2024/3/PAC2_2#Customer> "Customer")
SubClassOf(<http://www.semanticweb.org/dani2/ontologies/2024/3/PAC2_2#Customer> <http://www.semanticweb.org/dani2/ontologies/2024/3/PAC2_2#Flight>)
SubClassOf(<http://www.semanticweb.org/dani2/ontologies/2024/3/PAC2_2#Customer> ObjectSomeValuesFrom(<http://www.semanticweb.org/dani2/ontologies/2024/3/PAC2_2#hasCustomer> <http://www.semanticweb.org/dani2/ontologies/2024/3/PAC2_2#Traveller>))

# Class: <http://www.semanticweb.org/dani2/ontologies/2024/3/PAC2_2#Customer_Flight_Review> (<http://www.semanticweb.org/dani2/ontologies/2024/3/PAC2_2#Customer_Flight_Review>)

AnnotationAssertion(rdfs:comment <http://www.semanticweb.org/dani2/ontologies/2024/3/PAC2_2#Customer_Flight_Review> "A review performed by a customer on a flight service.")
SubClassOf(<http://www.semanticweb.org/dani2/ontologies/2024/3/PAC2_2#Customer_Flight_Review> <http://www.semanticweb.org/dani2/ontologies/2024/3/PAC2_2#Customer_Review>)

# Class: <http://www.semanticweb.org/dani2/ontologies/2024/3/PAC2_2#Customer_Review> (Customer Review)

AnnotationAssertion(rdfs:comment <http://www.semanticweb.org/dani2/ontologies/2024/3/PAC2_2#Customer_Review> "A review performed by a customer.")
AnnotationAssertion(rdfs:label <http://www.semanticweb.org/dani2/ontologies/2024/3/PAC2_2#Customer_Review> "Customer Review")
SubClassOf(<http://www.semanticweb.org/dani2/ontologies/2024/3/PAC2_2#Customer_Review> <http://www.semanticweb.org/dani2/ontologies/2024/3/PAC2_2#Review>)
DisjointClasses(<http://www.semanticweb.org/dani2/ontologies/2024/3/PAC2_2#Customer_Review> <http://www.semanticweb.org/dani2/ontologies/2024/3/PAC2_2#Professional_Review>)

# Class: <http://www.semanticweb.org/dani2/ontologies/2024/3/PAC2_2#Date> (Date)

AnnotationAssertion(rdfs:comment <http://www.semanticweb.org/dani2/ontologies/2024/3/PAC2_2#Date> "A date")
AnnotationAssertion(rdfs:label <http://www.semanticweb.org/dani2/ontologies/2024/3/PAC2_2#Date> "Date")
AnnotationAssertion(rdfs:sameAs <http://www.semanticweb.org/dani2/ontologies/2024/3/PAC2_2#Date> "https://dbpedia.org/page/Date")

# Class: <http://www.semanticweb.org/dani2/ontologies/2024/3/PAC2_2#Day> (Day)

AnnotationAssertion(rdfs:comment <http://www.semanticweb.org/dani2/ontologies/2024/3/PAC2_2#Day> "A day of the month")
AnnotationAssertion(rdfs:label <http://www.semanticweb.org/dani2/ontologies/2024/3/PAC2_2#Day> "Day")
SubClassOf(<http://www.semanticweb.org/dani2/ontologies/2024/3/PAC2_2#Day> <http://www.semanticweb.org/dani2/ontologies/2024/3/PAC2_2#Date>)

# Class: <http://www.semanticweb.org/dani2/ontologies/2024/3/PAC2_2#Description> (Description)

AnnotationAssertion(rdfs:comment <http://www.semanticweb.org/dani2/ontologies/2024/3/PAC2_2#Description> "A description to provide details of the review performed")
AnnotationAssertion(rdfs:label <http://www.semanticweb.org/dani2/ontologies/2024/3/PAC2_2#Description> "Description")
SubClassOf(<http://www.semanticweb.org/dani2/ontologies/2024/3/PAC2_2#Description> <http://www.semanticweb.org/dani2/ontologies/2024/3/PAC2_2#Customer_Flight_Review>)

# Class: <http://www.semanticweb.org/dani2/ontologies/2024/3/PAC2_2#Destination> (Destination)

AnnotationAssertion(rdfs:comment <http://www.semanticweb.org/dani2/ontologies/2024/3/PAC2_2#Destination> "A city where the airplane is supposed to arrive at the end of the flight.")
AnnotationAssertion(rdfs:label <http://www.semanticweb.org/dani2/ontologies/2024/3/PAC2_2#Destination> "Destination")
SubClassOf(<http://www.semanticweb.org/dani2/ontologies/2024/3/PAC2_2#Destination> <http://www.semanticweb.org/dani2/ontologies/2024/3/PAC2_2#Flight>)
SubClassOf(<http://www.semanticweb.org/dani2/ontologies/2024/3/PAC2_2#Destination> ObjectExactCardinality(1 <http://www.semanticweb.org/dani2/ontologies/2024/3/PAC2_2#hasDestination> <http://www.semanticweb.org/dani2/ontologies/2024/3/PAC2_2#City>))

# Class: <http://www.semanticweb.org/dani2/ontologies/2024/3/PAC2_2#EconomyClass> (EconomyClass)

AnnotationAssertion(rdfs:comment <http://www.semanticweb.org/dani2/ontologies/2024/3/PAC2_2#EconomyClass> "Seats with the lowest price")
AnnotationAssertion(rdfs:label <http://www.semanticweb.org/dani2/ontologies/2024/3/PAC2_2#EconomyClass> "EconomyClass")
SubClassOf(<http://www.semanticweb.org/dani2/ontologies/2024/3/PAC2_2#EconomyClass> <http://www.semanticweb.org/dani2/ontologies/2024/3/PAC2_2#SeatClass>)

# Class: <http://www.semanticweb.org/dani2/ontologies/2024/3/PAC2_2#Family_Leisure> (Family Leisure)

AnnotationAssertion(rdfs:comment <http://www.semanticweb.org/dani2/ontologies/2024/3/PAC2_2#Family_Leisure> "Travellers that are travelling with their family.")
AnnotationAssertion(rdfs:label <http://www.semanticweb.org/dani2/ontologies/2024/3/PAC2_2#Family_Leisure> "Family Leisure")
SubClassOf(<http://www.semanticweb.org/dani2/ontologies/2024/3/PAC2_2#Family_Leisure> <http://www.semanticweb.org/dani2/ontologies/2024/3/PAC2_2#Leisure_Traveller>)
DisjointClasses(<http://www.semanticweb.org/dani2/ontologies/2024/3/PAC2_2#Family_Leisure> <http://www.semanticweb.org/dani2/ontologies/2024/3/PAC2_2#Solo_Leisure>)

# Class: <http://www.semanticweb.org/dani2/ontologies/2024/3/PAC2_2#FirstClass> (FirstClass)

AnnotationAssertion(rdfs:comment <http://www.semanticweb.org/dani2/ontologies/2024/3/PAC2_2#FirstClass> "Premium seat class")
AnnotationAssertion(rdfs:label <http://www.semanticweb.org/dani2/ontologies/2024/3/PAC2_2#FirstClass> "FirstClass")
SubClassOf(<http://www.semanticweb.org/dani2/ontologies/2024/3/PAC2_2#FirstClass> <http://www.semanticweb.org/dani2/ontologies/2024/3/PAC2_2#SeatClass>)

# Class: <http://www.semanticweb.org/dani2/ontologies/2024/3/PAC2_2#Flight> (Flight)

AnnotationAssertion(rdfs:comment <http://www.semanticweb.org/dani2/ontologies/2024/3/PAC2_2#Flight> "A flight between two cities")
AnnotationAssertion(rdfs:label <http://www.semanticweb.org/dani2/ontologies/2024/3/PAC2_2#Flight> "Flight")
SubClassOf(<http://www.semanticweb.org/dani2/ontologies/2024/3/PAC2_2#Flight> <http://www.semanticweb.org/dani2/ontologies/2024/3/PAC2_2#Flight_Service>)

# Class: <http://www.semanticweb.org/dani2/ontologies/2024/3/PAC2_2#Flight_Date> (Flight Date)

AnnotationAssertion(rdfs:comment <http://www.semanticweb.org/dani2/ontologies/2024/3/PAC2_2#Flight_Date> "Date of the flight")
AnnotationAssertion(rdfs:label <http://www.semanticweb.org/dani2/ontologies/2024/3/PAC2_2#Flight_Date> "Flight Date")
SubClassOf(<http://www.semanticweb.org/dani2/ontologies/2024/3/PAC2_2#Flight_Date> <http://www.semanticweb.org/dani2/ontologies/2024/3/PAC2_2#Flight>)

# Class: <http://www.semanticweb.org/dani2/ontologies/2024/3/PAC2_2#Flight_Rate> (Flight Rate)

AnnotationAssertion(rdfs:comment <http://www.semanticweb.org/dani2/ontologies/2024/3/PAC2_2#Flight_Rate> "A rate to calificate the flight service.")
AnnotationAssertion(rdfs:label <http://www.semanticweb.org/dani2/ontologies/2024/3/PAC2_2#Flight_Rate> "Flight Rate")
SubClassOf(<http://www.semanticweb.org/dani2/ontologies/2024/3/PAC2_2#Flight_Rate> <http://www.semanticweb.org/dani2/ontologies/2024/3/PAC2_2#Customer_Flight_Review>)

# Class: <http://www.semanticweb.org/dani2/ontologies/2024/3/PAC2_2#Flight_Service> (Flight Service)

AnnotationAssertion(rdfs:comment <http://www.semanticweb.org/dani2/ontologies/2024/3/PAC2_2#Flight_Service> "A flight service provided")
AnnotationAssertion(rdfs:label <http://www.semanticweb.org/dani2/ontologies/2024/3/PAC2_2#Flight_Service> "Flight Service")
SubClassOf(<http://www.semanticweb.org/dani2/ontologies/2024/3/PAC2_2#Flight_Service> <http://www.semanticweb.org/dani2/ontologies/2024/3/PAC2_2#Services>)

# Class: <http://www.semanticweb.org/dani2/ontologies/2024/3/PAC2_2#Leisure_Traveller> (Leisure Traveller)

AnnotationAssertion(rdfs:comment <http://www.semanticweb.org/dani2/ontologies/2024/3/PAC2_2#Leisure_Traveller> "Traveller that has leisure as their purpouse.")
AnnotationAssertion(rdfs:label <http://www.semanticweb.org/dani2/ontologies/2024/3/PAC2_2#Leisure_Traveller> "Leisure Traveller")
SubClassOf(<http://www.semanticweb.org/dani2/ontologies/2024/3/PAC2_2#Leisure_Traveller> <http://www.semanticweb.org/dani2/ontologies/2024/3/PAC2_2#Traveller>)

# Class: <http://www.semanticweb.org/dani2/ontologies/2024/3/PAC2_2#Month> (Month)

AnnotationAssertion(rdfs:comment <http://www.semanticweb.org/dani2/ontologies/2024/3/PAC2_2#Month> "A month of the year")
AnnotationAssertion(rdfs:label <http://www.semanticweb.org/dani2/ontologies/2024/3/PAC2_2#Month> "Month")
SubClassOf(<http://www.semanticweb.org/dani2/ontologies/2024/3/PAC2_2#Month> <http://www.semanticweb.org/dani2/ontologies/2024/3/PAC2_2#Date>)

# Class: <http://www.semanticweb.org/dani2/ontologies/2024/3/PAC2_2#Nationality> (Nationality)

AnnotationAssertion(rdfs:comment <http://www.semanticweb.org/dani2/ontologies/2024/3/PAC2_2#Nationality> "Country of birth of the person")
AnnotationAssertion(rdfs:label <http://www.semanticweb.org/dani2/ontologies/2024/3/PAC2_2#Nationality> "Nationality")
SubClassOf(<http://www.semanticweb.org/dani2/ontologies/2024/3/PAC2_2#Nationality> <http://www.semanticweb.org/dani2/ontologies/2024/3/PAC2_2#Person>)

# Class: <http://www.semanticweb.org/dani2/ontologies/2024/3/PAC2_2#No> (No)

AnnotationAssertion(rdfs:comment <http://www.semanticweb.org/dani2/ontologies/2024/3/PAC2_2#No> "No")
AnnotationAssertion(rdfs:label <http://www.semanticweb.org/dani2/ontologies/2024/3/PAC2_2#No> "No")
SubClassOf(<http://www.semanticweb.org/dani2/ontologies/2024/3/PAC2_2#No> <http://www.semanticweb.org/dani2/ontologies/2024/3/PAC2_2#Recommend>)
DisjointClasses(<http://www.semanticweb.org/dani2/ontologies/2024/3/PAC2_2#No> <http://www.semanticweb.org/dani2/ontologies/2024/3/PAC2_2#Yes>)
DisjointClasses(<http://www.semanticweb.org/dani2/ontologies/2024/3/PAC2_2#No> <http://www.semanticweb.org/dani2/ontologies/2024/3/PAC2_2#N/A>)

# Class: <http://www.semanticweb.org/dani2/ontologies/2024/3/PAC2_2#Origin> (Origin)

AnnotationAssertion(rdfs:comment <http://www.semanticweb.org/dani2/ontologies/2024/3/PAC2_2#Origin> "The city from where the airplanes starts its flight.")
AnnotationAssertion(rdfs:label <http://www.semanticweb.org/dani2/ontologies/2024/3/PAC2_2#Origin> "Origin")
SubClassOf(<http://www.semanticweb.org/dani2/ontologies/2024/3/PAC2_2#Origin> <http://www.semanticweb.org/dani2/ontologies/2024/3/PAC2_2#Flight>)
SubClassOf(<http://www.semanticweb.org/dani2/ontologies/2024/3/PAC2_2#Origin> ObjectExactCardinality(1 <http://www.semanticweb.org/dani2/ontologies/2024/3/PAC2_2#hasOrigin> <http://www.semanticweb.org/dani2/ontologies/2024/3/PAC2_2#City>))

# Class: <http://www.semanticweb.org/dani2/ontologies/2024/3/PAC2_2#Owner> (Owner)

AnnotationAssertion(rdfs:comment <http://www.semanticweb.org/dani2/ontologies/2024/3/PAC2_2#Owner> "Company owner of the flight provided.")
AnnotationAssertion(rdfs:label <http://www.semanticweb.org/dani2/ontologies/2024/3/PAC2_2#Owner> "Owner")
SubClassOf(<http://www.semanticweb.org/dani2/ontologies/2024/3/PAC2_2#Owner> <http://www.semanticweb.org/dani2/ontologies/2024/3/PAC2_2#Flight>)
SubClassOf(<http://www.semanticweb.org/dani2/ontologies/2024/3/PAC2_2#Owner> ObjectExactCardinality(1 <http://www.semanticweb.org/dani2/ontologies/2024/3/PAC2_2#hasOwner> <http://www.semanticweb.org/dani2/ontologies/2024/3/PAC2_2#Airline_Company>))

# Class: <http://www.semanticweb.org/dani2/ontologies/2024/3/PAC2_2#Person> (Person)

AnnotationAssertion(rdfs:label <http://www.semanticweb.org/dani2/ontologies/2024/3/PAC2_2#Person> "Person")

# Class: <http://www.semanticweb.org/dani2/ontologies/2024/3/PAC2_2#PremiunEconomyClass> (PremiumEconomyClass)

AnnotationAssertion(rdfs:comment <http://www.semanticweb.org/dani2/ontologies/2024/3/PAC2_2#PremiunEconomyClass> "Economic seats but with some more space")
AnnotationAssertion(rdfs:label <http://www.semanticweb.org/dani2/ontologies/2024/3/PAC2_2#PremiunEconomyClass> "PremiumEconomyClass")
SubClassOf(<http://www.semanticweb.org/dani2/ontologies/2024/3/PAC2_2#PremiunEconomyClass> <http://www.semanticweb.org/dani2/ontologies/2024/3/PAC2_2#SeatClass>)

# Class: <http://www.semanticweb.org/dani2/ontologies/2024/3/PAC2_2#Professional_Review> (Professional Review)

AnnotationAssertion(rdfs:comment <http://www.semanticweb.org/dani2/ontologies/2024/3/PAC2_2#Professional_Review> "A review performed by a professional.")
AnnotationAssertion(rdfs:label <http://www.semanticweb.org/dani2/ontologies/2024/3/PAC2_2#Professional_Review> "Professional Review")
SubClassOf(<http://www.semanticweb.org/dani2/ontologies/2024/3/PAC2_2#Professional_Review> <http://www.semanticweb.org/dani2/ontologies/2024/3/PAC2_2#Review>)

# Class: <http://www.semanticweb.org/dani2/ontologies/2024/3/PAC2_2#Recommend> (Recommend)

AnnotationAssertion(rdfs:comment <http://www.semanticweb.org/dani2/ontologies/2024/3/PAC2_2#Recommend> "Whether a customer would recommend or not a flight")
AnnotationAssertion(rdfs:label <http://www.semanticweb.org/dani2/ontologies/2024/3/PAC2_2#Recommend> "Recommend")
SubClassOf(<http://www.semanticweb.org/dani2/ontologies/2024/3/PAC2_2#Recommend> <http://www.semanticweb.org/dani2/ontologies/2024/3/PAC2_2#Customer_Flight_Review>)

# Class: <http://www.semanticweb.org/dani2/ontologies/2024/3/PAC2_2#Review> (Review)

AnnotationAssertion(rdfs:comment <http://www.semanticweb.org/dani2/ontologies/2024/3/PAC2_2#Review> "A review performed")
AnnotationAssertion(rdfs:label <http://www.semanticweb.org/dani2/ontologies/2024/3/PAC2_2#Review> "Review")

# Class: <http://www.semanticweb.org/dani2/ontologies/2024/3/PAC2_2#Review_Owner> (Review Owner)

AnnotationAssertion(rdfs:comment <http://www.semanticweb.org/dani2/ontologies/2024/3/PAC2_2#Review_Owner> "The owner of the review")
AnnotationAssertion(rdfs:label <http://www.semanticweb.org/dani2/ontologies/2024/3/PAC2_2#Review_Owner> "Review Owner")
SubClassOf(<http://www.semanticweb.org/dani2/ontologies/2024/3/PAC2_2#Review_Owner> <http://www.semanticweb.org/dani2/ontologies/2024/3/PAC2_2#Customer_Flight_Review>)

# Class: <http://www.semanticweb.org/dani2/ontologies/2024/3/PAC2_2#SeatClass> (SeatClass)

AnnotationAssertion(rdfs:comment <http://www.semanticweb.org/dani2/ontologies/2024/3/PAC2_2#SeatClass> "Class of the seat")
AnnotationAssertion(rdfs:label <http://www.semanticweb.org/dani2/ontologies/2024/3/PAC2_2#SeatClass> "SeatClass")
SubClassOf(<http://www.semanticweb.org/dani2/ontologies/2024/3/PAC2_2#SeatClass> <http://www.semanticweb.org/dani2/ontologies/2024/3/PAC2_2#Customer_Flight_Review>)

# Class: <http://www.semanticweb.org/dani2/ontologies/2024/3/PAC2_2#Services> (Services)

AnnotationAssertion(rdfs:comment <http://www.semanticweb.org/dani2/ontologies/2024/3/PAC2_2#Services> "All the services that are owned by the airplane ccompany")
AnnotationAssertion(rdfs:label <http://www.semanticweb.org/dani2/ontologies/2024/3/PAC2_2#Services> "Services")
SubClassOf(<http://www.semanticweb.org/dani2/ontologies/2024/3/PAC2_2#Services> <http://www.semanticweb.org/dani2/ontologies/2024/3/PAC2_2#Airline_Company>)

# Class: <http://www.semanticweb.org/dani2/ontologies/2024/3/PAC2_2#Solo_Leisure> (Solo Leisure)

AnnotationAssertion(rdfs:comment <http://www.semanticweb.org/dani2/ontologies/2024/3/PAC2_2#Solo_Leisure> "Travellers that are travelling alone.")
AnnotationAssertion(rdfs:label <http://www.semanticweb.org/dani2/ontologies/2024/3/PAC2_2#Solo_Leisure> "Solo Leisure")
SubClassOf(<http://www.semanticweb.org/dani2/ontologies/2024/3/PAC2_2#Solo_Leisure> <http://www.semanticweb.org/dani2/ontologies/2024/3/PAC2_2#Leisure_Traveller>)

# Class: <http://www.semanticweb.org/dani2/ontologies/2024/3/PAC2_2#Ticket> (Ticket)

AnnotationAssertion(rdfs:comment <http://www.semanticweb.org/dani2/ontologies/2024/3/PAC2_2#Ticket> "Item to be sold to the customers of the flight, that allows the person to use the service.")
AnnotationAssertion(rdfs:label <http://www.semanticweb.org/dani2/ontologies/2024/3/PAC2_2#Ticket> "Ticket")
SubClassOf(<http://www.semanticweb.org/dani2/ontologies/2024/3/PAC2_2#Ticket> <http://www.semanticweb.org/dani2/ontologies/2024/3/PAC2_2#Flight>)

# Class: <http://www.semanticweb.org/dani2/ontologies/2024/3/PAC2_2#Title> (Title)

AnnotationAssertion(rdfs:comment <http://www.semanticweb.org/dani2/ontologies/2024/3/PAC2_2#Title> "A title to summarize the review")
AnnotationAssertion(rdfs:label <http://www.semanticweb.org/dani2/ontologies/2024/3/PAC2_2#Title> "Title")
SubClassOf(<http://www.semanticweb.org/dani2/ontologies/2024/3/PAC2_2#Title> <http://www.semanticweb.org/dani2/ontologies/2024/3/PAC2_2#Customer_Flight_Review>)

# Class: <http://www.semanticweb.org/dani2/ontologies/2024/3/PAC2_2#Traveller> (Traveller)

AnnotationAssertion(rdfs:comment <http://www.semanticweb.org/dani2/ontologies/2024/3/PAC2_2#Traveller> "Person that is travelling")
AnnotationAssertion(rdfs:label <http://www.semanticweb.org/dani2/ontologies/2024/3/PAC2_2#Traveller> "Traveller")
SubClassOf(<http://www.semanticweb.org/dani2/ontologies/2024/3/PAC2_2#Traveller> <http://www.semanticweb.org/dani2/ontologies/2024/3/PAC2_2#Person>)

# Class: <http://www.semanticweb.org/dani2/ontologies/2024/3/PAC2_2#Vehicle> (Vehicle)

AnnotationAssertion(rdfs:comment <http://www.semanticweb.org/dani2/ontologies/2024/3/PAC2_2#Vehicle> "A vehicle")
AnnotationAssertion(rdfs:label <http://www.semanticweb.org/dani2/ontologies/2024/3/PAC2_2#Vehicle> "Vehicle")

# Class: <http://www.semanticweb.org/dani2/ontologies/2024/3/PAC2_2#Year> (Year)

AnnotationAssertion(rdfs:comment <http://www.semanticweb.org/dani2/ontologies/2024/3/PAC2_2#Year> "A year")
AnnotationAssertion(rdfs:label <http://www.semanticweb.org/dani2/ontologies/2024/3/PAC2_2#Year> "Year")
SubClassOf(<http://www.semanticweb.org/dani2/ontologies/2024/3/PAC2_2#Year> <http://www.semanticweb.org/dani2/ontologies/2024/3/PAC2_2#Date>)

# Class: <http://www.semanticweb.org/dani2/ontologies/2024/3/PAC2_2#Yes> (Yes)

AnnotationAssertion(rdfs:comment <http://www.semanticweb.org/dani2/ontologies/2024/3/PAC2_2#Yes> "Yes")
AnnotationAssertion(rdfs:label <http://www.semanticweb.org/dani2/ontologies/2024/3/PAC2_2#Yes> "Yes")
SubClassOf(<http://www.semanticweb.org/dani2/ontologies/2024/3/PAC2_2#Yes> <http://www.semanticweb.org/dani2/ontologies/2024/3/PAC2_2#Recommend>)
DisjointClasses(<http://www.semanticweb.org/dani2/ontologies/2024/3/PAC2_2#Yes> <http://www.semanticweb.org/dani2/ontologies/2024/3/PAC2_2#N/A>)

# Class: <http://www.semanticweb.org/dani2/ontologies/2024/3/PAC2_2#N/A> (N/A)

AnnotationAssertion(rdfs:comment <http://www.semanticweb.org/dani2/ontologies/2024/3/PAC2_2#N/A> "Not applicable")
AnnotationAssertion(rdfs:label <http://www.semanticweb.org/dani2/ontologies/2024/3/PAC2_2#N/A> "N/A")
SubClassOf(<http://www.semanticweb.org/dani2/ontologies/2024/3/PAC2_2#N/A> <http://www.semanticweb.org/dani2/ontologies/2024/3/PAC2_2#Recommend>)


############################
#   Named Individuals
############################

# Individual: <http://www.semanticweb.org/dani2/ontologies/2024/3/PAC2_2#Albert> (Albert)

AnnotationAssertion(rdfs:comment <http://www.semanticweb.org/dani2/ontologies/2024/3/PAC2_2#Albert> "A person.")
AnnotationAssertion(rdfs:label <http://www.semanticweb.org/dani2/ontologies/2024/3/PAC2_2#Albert> "Albert")
ClassAssertion(<http://www.semanticweb.org/dani2/ontologies/2024/3/PAC2_2#Person> <http://www.semanticweb.org/dani2/ontologies/2024/3/PAC2_2#Albert>)
ObjectPropertyAssertion(<http://www.semanticweb.org/dani2/ontologies/2024/3/PAC2_2#hasFlight> <http://www.semanticweb.org/dani2/ontologies/2024/3/PAC2_2#Albert> <http://www.semanticweb.org/dani2/ontologies/2024/3/PAC2_2#Boeing737_Albacete_Standsted_13/12/22>)
DataPropertyAssertion(<http://www.semanticweb.org/dani2/ontologies/2024/3/PAC2_2#hasRating> <http://www.semanticweb.org/dani2/ontologies/2024/3/PAC2_2#Albert> "6"^^xsd:integer)

# Individual: <http://www.semanticweb.org/dani2/ontologies/2024/3/PAC2_2#Alicante> (Albacete)

AnnotationAssertion(rdfs:comment <http://www.semanticweb.org/dani2/ontologies/2024/3/PAC2_2#Alicante> "A city")
AnnotationAssertion(rdfs:label <http://www.semanticweb.org/dani2/ontologies/2024/3/PAC2_2#Alicante> "Albacete")
ClassAssertion(<http://www.semanticweb.org/dani2/ontologies/2024/3/PAC2_2#City> <http://www.semanticweb.org/dani2/ontologies/2024/3/PAC2_2#Alicante>)

# Individual: <http://www.semanticweb.org/dani2/ontologies/2024/3/PAC2_2#Boeing_737> (Boeing 737)

AnnotationAssertion(rdfs:comment <http://www.semanticweb.org/dani2/ontologies/2024/3/PAC2_2#Boeing_737> "Vuelo Boeing 737 del 13/12/2022 organizado por la compa√±ia Ryanair.")
AnnotationAssertion(rdfs:label <http://www.semanticweb.org/dani2/ontologies/2024/3/PAC2_2#Boeing_737> "Boeing 737")
ClassAssertion(<http://www.semanticweb.org/dani2/ontologies/2024/3/PAC2_2#Airplane> <http://www.semanticweb.org/dani2/ontologies/2024/3/PAC2_2#Boeing_737>)

# Individual: <http://www.semanticweb.org/dani2/ontologies/2024/3/PAC2_2#David> (David)

AnnotationAssertion(rdfs:comment <http://www.semanticweb.org/dani2/ontologies/2024/3/PAC2_2#David> "A person")
AnnotationAssertion(rdfs:label <http://www.semanticweb.org/dani2/ontologies/2024/3/PAC2_2#David> "David")
ClassAssertion(<http://www.semanticweb.org/dani2/ontologies/2024/3/PAC2_2#Person> <http://www.semanticweb.org/dani2/ontologies/2024/3/PAC2_2#David>)
DataPropertyAssertion(<http://www.semanticweb.org/dani2/ontologies/2024/3/PAC2_2#hasAge> <http://www.semanticweb.org/dani2/ontologies/2024/3/PAC2_2#David> "28"^^xsd:integer)
DataPropertyAssertion(<http://www.semanticweb.org/dani2/ontologies/2024/3/PAC2_2#hasRating> <http://www.semanticweb.org/dani2/ontologies/2024/3/PAC2_2#David> "7"^^xsd:integer)

# Individual: <http://www.semanticweb.org/dani2/ontologies/2024/3/PAC2_2#Marta> (Marta)

AnnotationAssertion(rdfs:comment <http://www.semanticweb.org/dani2/ontologies/2024/3/PAC2_2#Marta> "A person")
AnnotationAssertion(rdfs:label <http://www.semanticweb.org/dani2/ontologies/2024/3/PAC2_2#Marta> "Marta")
ClassAssertion(<http://www.semanticweb.org/dani2/ontologies/2024/3/PAC2_2#Person> <http://www.semanticweb.org/dani2/ontologies/2024/3/PAC2_2#Marta>)
ObjectPropertyAssertion(<http://www.semanticweb.org/dani2/ontologies/2024/3/PAC2_2#hasSeatClass> <http://www.semanticweb.org/dani2/ontologies/2024/3/PAC2_2#Marta> <http://www.semanticweb.org/dani2/ontologies/2024/3/PAC2_2#Seat2A>)

# Individual: <http://www.semanticweb.org/dani2/ontologies/2024/3/PAC2_2#Ryanair> (Ryanair)

AnnotationAssertion(rdfs:comment <http://www.semanticweb.org/dani2/ontologies/2024/3/PAC2_2#Ryanair> "An airplane company")
AnnotationAssertion(rdfs:label <http://www.semanticweb.org/dani2/ontologies/2024/3/PAC2_2#Ryanair> "Ryanair")
ClassAssertion(<http://www.semanticweb.org/dani2/ontologies/2024/3/PAC2_2#Airline_Company> <http://www.semanticweb.org/dani2/ontologies/2024/3/PAC2_2#Ryanair>)

# Individual: <http://www.semanticweb.org/dani2/ontologies/2024/3/PAC2_2#Seat13B> (Seat13B)

AnnotationAssertion(rdfs:comment <http://www.semanticweb.org/dani2/ontologies/2024/3/PAC2_2#Seat13B> "A seat of a airplane")
AnnotationAssertion(rdfs:label <http://www.semanticweb.org/dani2/ontologies/2024/3/PAC2_2#Seat13B> "Seat13B")
ClassAssertion(<http://www.semanticweb.org/dani2/ontologies/2024/3/PAC2_2#EconomyClass> <http://www.semanticweb.org/dani2/ontologies/2024/3/PAC2_2#Seat13B>)

# Individual: <http://www.semanticweb.org/dani2/ontologies/2024/3/PAC2_2#Seat2A> (Seat2A)

AnnotationAssertion(rdfs:comment <http://www.semanticweb.org/dani2/ontologies/2024/3/PAC2_2#Seat2A> "A seat of a airplane")
AnnotationAssertion(rdfs:label <http://www.semanticweb.org/dani2/ontologies/2024/3/PAC2_2#Seat2A> "Seat2A")
ClassAssertion(<http://www.semanticweb.org/dani2/ontologies/2024/3/PAC2_2#FirstClass> <http://www.semanticweb.org/dani2/ontologies/2024/3/PAC2_2#Seat2A>)

# Individual: <http://www.semanticweb.org/dani2/ontologies/2024/3/PAC2_2#Standsted> (Standsted)

AnnotationAssertion(rdfs:comment <http://www.semanticweb.org/dani2/ontologies/2024/3/PAC2_2#Standsted> "A city.")
AnnotationAssertion(rdfs:label <http://www.semanticweb.org/dani2/ontologies/2024/3/PAC2_2#Standsted> "Standsted")
ClassAssertion(<http://www.semanticweb.org/dani2/ontologies/2024/3/PAC2_2#City> <http://www.semanticweb.org/dani2/ontologies/2024/3/PAC2_2#Standsted>)

# Individual: <http://www.semanticweb.org/dani2/ontologies/2024/3/PAC2_2#13/12/2022> (13/12/2022)

AnnotationAssertion(rdfs:comment <http://www.semanticweb.org/dani2/ontologies/2024/3/PAC2_2#13/12/2022> "A date")
AnnotationAssertion(rdfs:label <http://www.semanticweb.org/dani2/ontologies/2024/3/PAC2_2#13/12/2022> "13/12/2022")
ClassAssertion(<http://www.semanticweb.org/dani2/ontologies/2024/3/PAC2_2#Date> <http://www.semanticweb.org/dani2/ontologies/2024/3/PAC2_2#13/12/2022>)

# Individual: <http://www.semanticweb.org/dani2/ontologies/2024/3/PAC2_2#Boeing737_Albacete_Standsted_13/12/22> (Boeing737 Albacete-Standsted 13/12/2022)

AnnotationAssertion(rdfs:comment <http://www.semanticweb.org/dani2/ontologies/2024/3/PAC2_2#Boeing737_Albacete_Standsted_13/12/22> "Flight Boeing 737 owned by Ryanair, with origin in Albacete and Standsted destination. On 13/12/2022.")
AnnotationAssertion(rdfs:label <http://www.semanticweb.org/dani2/ontologies/2024/3/PAC2_2#Boeing737_Albacete_Standsted_13/12/22> "Boeing737 Albacete-Standsted 13/12/2022")
ClassAssertion(<http://www.semanticweb.org/dani2/ontologies/2024/3/PAC2_2#Flight> <http://www.semanticweb.org/dani2/ontologies/2024/3/PAC2_2#Boeing737_Albacete_Standsted_13/12/22>)
ObjectPropertyAssertion(<http://www.semanticweb.org/dani2/ontologies/2024/3/PAC2_2#hasAirplane> <http://www.semanticweb.org/dani2/ontologies/2024/3/PAC2_2#Boeing737_Albacete_Standsted_13/12/22> <http://www.semanticweb.org/dani2/ontologies/2024/3/PAC2_2#Boeing_737>)
ObjectPropertyAssertion(<http://www.semanticweb.org/dani2/ontologies/2024/3/PAC2_2#hasCustomer> <http://www.semanticweb.org/dani2/ontologies/2024/3/PAC2_2#Boeing737_Albacete_Standsted_13/12/22> <http://www.semanticweb.org/dani2/ontologies/2024/3/PAC2_2#David>)
ObjectPropertyAssertion(<http://www.semanticweb.org/dani2/ontologies/2024/3/PAC2_2#hasCustomer> <http://www.semanticweb.org/dani2/ontologies/2024/3/PAC2_2#Boeing737_Albacete_Standsted_13/12/22> <http://www.semanticweb.org/dani2/ontologies/2024/3/PAC2_2#Marta>)
ObjectPropertyAssertion(<http://www.semanticweb.org/dani2/ontologies/2024/3/PAC2_2#hasDestination> <http://www.semanticweb.org/dani2/ontologies/2024/3/PAC2_2#Boeing737_Albacete_Standsted_13/12/22> <http://www.semanticweb.org/dani2/ontologies/2024/3/PAC2_2#Standsted>)
ObjectPropertyAssertion(<http://www.semanticweb.org/dani2/ontologies/2024/3/PAC2_2#hasFlightDate> <http://www.semanticweb.org/dani2/ontologies/2024/3/PAC2_2#Boeing737_Albacete_Standsted_13/12/22> <http://www.semanticweb.org/dani2/ontologies/2024/3/PAC2_2#13/12/2022>)
ObjectPropertyAssertion(<http://www.semanticweb.org/dani2/ontologies/2024/3/PAC2_2#hasOrigin> <http://www.semanticweb.org/dani2/ontologies/2024/3/PAC2_2#Boeing737_Albacete_Standsted_13/12/22> <http://www.semanticweb.org/dani2/ontologies/2024/3/PAC2_2#Alicante>)
ObjectPropertyAssertion(<http://www.semanticweb.org/dani2/ontologies/2024/3/PAC2_2#hasOwner> <http://www.semanticweb.org/dani2/ontologies/2024/3/PAC2_2#Boeing737_Albacete_Standsted_13/12/22> <http://www.semanticweb.org/dani2/ontologies/2024/3/PAC2_2#Ryanair>)


DLSafeRule(Body(ObjectPropertyAtom(<http://www.semanticweb.org/dani2/ontologies/2024/3/PAC2_2#hasSeatClass> Variable(<urn:swrl:var#c>) Variable(<urn:swrl:var#FirstClass>)) ClassAtom(<http://www.semanticweb.org/dani2/ontologies/2024/3/PAC2_2#Review> Variable(<urn:swrl:var#c>)))Head(ClassAtom(<http://www.semanticweb.org/dani2/ontologies/2024/3/PAC2_2#Yes> Variable(<urn:swrl:var#c>))))
DLSafeRule(Body(ClassAtom(<http://www.semanticweb.org/dani2/ontologies/2024/3/PAC2_2#Review> Variable(<urn:swrl:var#c>)) DataPropertyAtom(<http://www.semanticweb.org/dani2/ontologies/2024/3/PAC2_2#hasRating> Variable(<urn:swrl:var#c>) Variable(<urn:swrl:var#n>)) BuiltInAtom(<http://www.w3.org/2003/11/swrlb#greaterThan> Variable(<urn:swrl:var#n>) "5"^^xsd:integer))Head(ClassAtom(<http://www.semanticweb.org/dani2/ontologies/2024/3/PAC2_2#Yes> Variable(<urn:swrl:var#c>))))
DLSafeRule(Body(ClassAtom(<http://www.semanticweb.org/dani2/ontologies/2024/3/PAC2_2#Review> Variable(<urn:swrl:var#c>)) DataPropertyAtom(<http://www.semanticweb.org/dani2/ontologies/2024/3/PAC2_2#hasRating> Variable(<urn:swrl:var#c>) Variable(<urn:swrl:var#n>)) BuiltInAtom(<http://www.w3.org/2003/11/swrlb#lessThan> Variable(<urn:swrl:var#n>) "6"^^xsd:integer))Head(ClassAtom(<http://www.semanticweb.org/dani2/ontologies/2024/3/PAC2_2#No> Variable(<urn:swrl:var#c>))))
)